src/Provers.v
@@ -170,8 +170,8 @@ Section Grouper.
     match grps with
       | nil => [a :: g]
       | g' :: grps' => if in_seq g' a
-                         then (g' ++ a :: g) :: grps'
-                         else g' :: groupWith grps' g a
+                       then (g' ++ a :: g) :: grps'
+                       else g' :: groupWith grps' g a
     end.
 
   Fixpoint addEquality (ls : list (list A)) (a : A) (b : A) : list (list A) :=
@@ -347,17 +347,9 @@ Section TransitivityProver.
   Qed.
 
   Definition eqD_seq (e1 e2 : expr types) : bool :=
-    match typeof fs uvars vars e1 with
+    match expr_seq_dec e1 e2 with
+      | Some pf2 => true
       | None => false
-      | Some _ =>
-        match typeof fs uvars vars e2 with
-          | None => false
-          | Some _ =>
-            match expr_seq_dec e1 e2 with
-              | Some pf2 => true
-              | None => false
-            end
-        end
     end.
 
   Fixpoint transitivityLearn (sum : transitivity_summary) (hyps : list (expr types)) : transitivity_summary :=
@@ -429,8 +421,6 @@ Section TransitivityProver.
     destruct a; auto.
     revert H; case_eq (exprD fs uvars vars (Equal t a1 a2) tvProp); intros; try contradiction.
     simpl in *. apply addEquality_sound; eauto.
-    unfold eqD_seq.
-    intros.
     
     Focus 2.
 
